Fix well_sch_spec

Dataflow/WellFormed/Decide.v
@@ -4,7 +4,9 @@ Require Import Rustre.Dataflow.Syntax.
 Require Import Rustre.Dataflow.IsFree.
 Require Import Rustre.Dataflow.IsFree.Decide.
 Require Import Rustre.Dataflow.IsVariable.
+Require Import Rustre.Dataflow.IsVariable.Decide.
 Require Import Rustre.Dataflow.IsDefined.
+Require Import Rustre.Dataflow.IsDefined.Decide.
 Require Import Rustre.Dataflow.WellFormed.
 
 Require Import Rustre.Dataflow.Ordered.
@@ -25,38 +27,20 @@ Remark: This development is not formally part of the correctness proof.
  *)
 
 Module Type DECIDE
-       (Ids: IDS)
-       (Op : OPERATORS)
-       (Import Syn : SYNTAX Ids Op)
-       (IsF : ISFREE Ids Op Syn)
+       (Ids           : IDS)
+       (Op            : OPERATORS)
+       (Import Syn    : SYNTAX Ids Op)
+       (IsF           : ISFREE Ids Op Syn)
        (Import IsFDec : IsFree.Decide.DECIDE Ids Op Syn IsF)
-       (Import Ord : ORDERED Ids Op Syn)
-       (Import Mem : MEMORIES Ids Op Syn)
-       (Import IsD : ISDEFINED Ids Op Syn Mem)
-       (Import IsV : ISVARIABLE Ids Op Syn Mem IsD)
-       (Import NoD : NODUP Ids Op Syn Mem IsD IsV)
-       (Import Wef : WELLFORMED Ids Op Syn IsF Ord Mem IsD IsV NoD).
-  
-  Section Decide.
+       (Import Ord    : ORDERED Ids Op Syn)
+       (Import Mem    : MEMORIES Ids Op Syn)
+       (Import IsD    : ISDEFINED Ids Op Syn Mem)
+       (Import IsV    : ISVARIABLE Ids Op Syn Mem IsD)
+       (Import IsDDec : IsDefined.Decide.DECIDE Ids Op Syn Mem IsD)
+       (Import IsVDec : IsVariable.Decide.DECIDE Ids Op Syn Mem IsD IsV)
+       (Import NoD    : NODUP Ids Op Syn Mem IsD IsV)
+       (Import Wef    : WELLFORMED Ids Op Syn IsF Ord Mem IsD IsV NoD).
 
-  End Decide.
-
-End DECIDE.
-
-Module DecideFun
-       (Ids: IDS)
-       (Op : OPERATORS)
-       (Import Syn : SYNTAX Ids Op)
-       (IsF : ISFREE Ids Op Syn)
-       (Import IsFDec : IsFree.Decide.DECIDE Ids Op Syn IsF)
-       (Import Ord : ORDERED Ids Op Syn)
-       (Import Mem : MEMORIES Ids Op Syn)
-       (Import IsD : ISDEFINED Ids Op Syn Mem)
-       (Import IsV : ISVARIABLE Ids Op Syn Mem IsD)
-       (Import NoD : NODUP Ids Op Syn Mem IsD IsV)
-       (Import Wef : WELLFORMED Ids Op Syn IsF Ord Mem IsD IsV NoD)
-       <: DECIDE Ids Op Syn IsF IsFDec Ord Mem IsD IsV NoD Wef.
-  
   Section Decide.
 
     Variable mems : PS.t.
@@ -98,241 +82,263 @@ Module DecideFun
           now apply Hnin with (1:=H).
     Qed.
 
-    Definition check_eq (eq: equation) (acc: bool*PS.t*PS.t): bool*PS.t*PS.t :=
+    Definition check_eq (eq: equation) (acc: bool*PS.t*PS.t)
+      : bool*PS.t*PS.t :=
       match acc with
       | (true, defined, variables) =>
-        match eq with
-        | EqDef x ck e =>
-          ((PS.for_all (check_var defined variables)
-                       (free_in_caexp ck e PS.empty))
-             && (negb (PS.mem x defined)),
-           PS.add x defined, PS.add x variables)
-        | EqApp x ck f les _ =>
-          ((PS.for_all (check_var defined variables)
-                       (free_in_laexps ck les PS.empty))
-             && (negb (PS.mem x defined)),
-           PS.add x defined, PS.add x variables)
-        | EqFby x ck v e =>
-          ((PS.mem x mems && PS.for_all (check_var defined variables)
-                   (free_in_laexp ck e PS.empty))
-             && (negb (PS.mem x defined)),
-           PS.add x defined, variables)
+        match var_defined eq with
+        | x => ((PS.for_all (check_var defined variables)
+                            (free_in_equation eq PS.empty))
+                  && (negb (PS.mem x defined)),
+                PS.add x defined, variable_eq variables eq)
         end
       | (false, _, _) => (false, PS.empty, PS.empty)
       end.
 
-    Definition well_sch (argIns: list ident)(eqs: list equation) : bool :=
-      fst
-        (fst
-           (List.fold_right
-              check_eq
-              (true, PS.empty, fold_left (fun a b => PS.add b a) argIns PS.empty)
-              eqs)).
+    Definition well_sch (args: list ident) (eqs: list equation) : bool :=
+      fst (fst (List.fold_right check_eq
+                                (true,
+                                 PS.empty,
+                                 fold_left (fun a b => PS.add b a) args PS.empty)
+                                eqs)).
 
-    (* Lemma not_for_all_spec: *)
-(*       forall (s : PS.t) (f : BinNums.positive -> bool), *)
-(*         SetoidList.compat_bool PS.E.eq f -> *)
-(*         (PS.for_all f s = false <-> ~(PS.For_all (fun x : PS.elt => f x = true) s)). *)
-(*     Proof. *)
-(*       intros s f HSL. *)
-(*       split. *)
-(*       - intros Hfa HFa. *)
-(*         apply (PS.for_all_spec _ HSL) in HFa. *)
-(*         rewrite Hfa in HFa. *)
-(*         discriminate. *)
-(*       - intro HFa. *)
-(*         apply Bool.not_true_iff_false. *)
-(*         intro Hfa; apply HFa. *)
-(*         apply (PS.for_all_spec _ HSL). *)
-(*         assumption. *)
-(*     Qed. *)
+    Lemma not_for_all_spec:
+      forall (s : PS.t) (f : BinNums.positive -> bool),
+        SetoidList.compat_bool PS.E.eq f ->
+        (PS.for_all f s = false <-> ~(PS.For_all (fun x : PS.elt => f x = true) s)).
+    Proof.
+      intros s f HSL.
+      split.
+      - intros Hfa HFa.
+        apply (PS.for_all_spec _ HSL) in HFa.
+        rewrite Hfa in HFa.
+        discriminate.
+      - intro HFa.
+        apply Bool.not_true_iff_false.
+        intro Hfa; apply HFa.
+        apply (PS.for_all_spec _ HSL).
+        assumption.
+    Qed.
 
-(*     Lemma check_var_compat: *)
-(*       forall defined variables, *)
-(*         SetoidList.compat_bool PS.E.eq (check_var defined variables). *)
-(*     Proof. *)
-(*       intros defined variables x y Heq. *)
-(*       unfold PS.E.eq in Heq. *)
-(*       rewrite Heq. *)
-(*       reflexivity. *)
-(*     Qed. *)
+    Lemma check_var_compat:
+      forall defined variables,
+        SetoidList.compat_bool PS.E.eq (check_var defined variables).
+    Proof.
+      intros defined variables x y Heq.
+      unfold PS.E.eq in Heq.
+      rewrite Heq.
+      reflexivity.
+    Qed.
 
-(*     Lemma well_sch_pre_spec: *)
-(*       forall argIns eqs good defined variables, *)
-(*         (good, defined, variables) *)
-(*         = List.fold_right check_eq (true, PS.empty, fold_left (fun a b => PS.add b a) argIns PS.empty) eqs *)
-(*         -> *)
-(*         (good = true *)
-(*          -> (Is_well_sch mems argIns eqs *)
-(*             /\ (forall x, PS.In x defined <-> Is_defined_in_eqs x eqs) *)
-(*             /\ (forall x, PS.In x variables <-> Is_variable_in_eqs x eqs \/ In x argIns))) *)
-(*         /\ (good = false -> ~Is_well_sch mems argIns eqs). *)
-(*     Admitted. (* XXX: Stating that a decision procedure behaves as expected. Not used *) *)
-(*     (* *)
-(*   induction eqs as [|eq]. *)
-(*   - simpl; injection 1; intros HRv HRm; subst. *)
-(*     intuition; *)
-(*       repeat match goal with *)
-(*                | H: PS.In _ (PS.add _ _) |- _ => rewrite PS.add_spec in H; destruct H *)
-(*                | H: PS.In _ PS.empty |- _ => apply PS.empty_spec in H; *)
-(*                                              contradiction *)
-(*                | H: Is_defined_in _ nil |- _ => now inversion H *)
-(*                | H: Is_variable_in _ nil |- _ => now inversion H *)
-(*                | H1:good=true, H2:good=false |- _ => rewrite H1 in H2; discriminate *)
-(*                | |- _ => tauto *)
-(*              end. *)
-(*   - intros good defined variables HH. *)
-(*     simpl in HH. *)
-(*     destruct (List.fold_right check_eq (true, PS.empty, PS.add argIn PS.empty) eqs) *)
-(*       as [[good' defined'] variables'] eqn:Heq. *)
-(*     specialize IHeqs with good' defined' variables'. *)
-(*     pose proof (IHeqs (eq_refl (good', defined', variables'))) as IH; *)
-(*       clear IHeqs. *)
-(*     destruct IH as [IHt IHf]. *)
-(*     split; intro Hg; rewrite Hg in *; clear Hg. *)
-(*     + destruct eq; (* the horror... *) (* XXX: . was ; *) *)
-(*       (simpl in HH; *)
-(*        assert (good' = true) as IH *)
-(*            by (apply Bool.not_false_iff_true; *)
-(*                intro Hgf; rewrite Hgf in HH; *)
-(*                discriminate); *)
-(*        rewrite IH in HH; *)
-(*        apply IHt in IH; clear IHt IHf; *)
-(*        destruct IH as [Hwsch [Hidi Hivi]]; *)
-(*        symmetry in HH; *)
-(*        injection HH; *)
-(*        intros HRv HRd; rewrite <-HRv,<-HRd in *; clear HRv HRd HH; *)
-(*        intro Hcv; apply Bool.andb_true_iff in Hcv; *)
-(*          destruct Hcv as [Hcv Hnin]; *)
-(*          try (apply Bool.andb_true_iff in Hcv; *)
-(*                destruct Hcv as [Him Hcv]); *)
-(*          rewrite Bool.negb_true_iff, *)
-(*          <-PSF.not_mem_iff in Hnin; *)
-(*        rewrite PS.for_all_spec in Hcv; *)
-(*          [ |now apply check_var_compat]; *)
-(*        try rewrite PS.mem_spec in Him; *)
-(*        split; *)
-(*        [constructor; *)
-(*          try (exact Hwsch *)
-(*               || assumption *)
-(*               || (intro HH; apply Hidi in HH; contradiction)); *)
-(*         intros y Hy; *)
-(*           apply free_in_caexp_spec' in Hy *)
-(*           || apply free_in_laexp_spec' in Hy; *)
-(*           apply Hcv in Hy; *)
-(*           apply check_var_spec in Hy; *)
-(*           repeat progress match goal with *)
-(*           | H:_ /\ _ |- _ => destruct H *)
-(*           | |- _ /\ _ => split; intros *)
-(*           | H1:PS.In ?y ?mems -> _, H2:PS.In ?y ?mems |- _ => apply H1 in H2 *)
-(*           | |- ~Is_defined_in ?x _ => intro *)
-(*           | H1:~PS.In ?x defined', *)
-(*             H2:Is_defined_in ?x eqs |- _ => apply Hidi in H2; contradiction *)
-(*           | |- Is_variable_in ?x eqs => auto; apply Hivi *)
-(*           | _ => now intuition *)
-(*                           end |]; *)
-(*       (now rewrite <- Hivi; auto) || *)
-(*       split; intro x; split; intro HH; *)
-(*          (apply PS.add_spec in HH; *)
-(*            destruct HH as [HH|HH]; try (now subst; repeat constructor); []; *)
-(*            solve [ now apply Hidi in HH; constructor 2 *)
-(*                  | apply Hivi in HH; destruct HH as [HH | HH]; tauto || constructor; constructor 2; *)
-(*                    []; inversion_clear HH; (now constructor) || (now constructor 2) ]) *)
-(*          || (rewrite PS.add_spec, ?Hivi, ?Hidi; *)
-(*               apply Is_defined_in_cons in HH *)
-(*               || (destruct HH as [HH | HH]; try tauto; []; apply Is_variable_in_cons in HH); *)
-(*               destruct HH as [HH|HH]; inversion_clear HH; tauto) *)
-(*          || (apply Hivi in HH; try (destruct HH as [HH | HH]; tauto || left); constructor 2; apply HH) *)
-(*          || (rewrite Hivi; try (destruct HH as [HH | HH]; try tauto; []); *)
-(*              apply Is_variable_in_cons in HH; destruct HH as [HH|HH]; inversion HH; tauto)). *)
-(*     + destruct good'; [clear IHf| inversion 1; apply IHf; auto ]. *)
-(*       pose proof (IHt (eq_refl true)) as IH; clear IHt. *)
-(*       destruct IH as [Hwsch [Hidi Hivi]]. *)
-(*       destruct eq; *)
-(*         (simpl in HH; *)
-(*           injection HH; *)
-(*           intros HRd HRv Hcv; *)
-(*           rewrite HRd,HRv in *; *)
-(*           clear HRd HRv HH; *)
-(*           symmetry in Hcv; *)
-(*           repeat progress match goal with *)
-(*           | Hcv:PS.mem _ _ && _ = false |- _ => *)
-(*             apply Bool.andb_false_iff in Hcv; *)
-(*               destruct Hcv as [Hcv|Hcv]; *)
-(*               [ inversion 1; *)
-(*                 apply mem_spec_false in Hcv; *)
-(*                 contradiction *)
-(*               | rewrite not_for_all_spec in Hcv; *)
-(*                 [ |now apply check_var_compat] ] *)
-(*           | H:_ && negb _ = false |- _ => *)
-(*             apply Bool.andb_false_iff in Hcv; *)
-(*               destruct Hcv as [Hcv|Hcv]; *)
-(*               [rewrite not_for_all_spec in Hcv; *)
-(*                 [ |now apply check_var_compat] *)
-(*               | rewrite Bool.negb_false_iff in Hcv; *)
-(*                 rewrite PS.mem_spec in Hcv; *)
-(*                 apply Hidi in Hcv; *)
-(*                 inversion 1; *)
-(*                 contradiction ] *)
-(*           | Hcv:PS.mem _ _ && _ && _ = false |- _ => *)
-(*             apply Bool.andb_false_iff in Hcv; *)
-(*               destruct Hcv as [Hcv|Hcv]; *)
-(*               [|rewrite Bool.negb_false_iff in Hcv; *)
-(*                  rewrite PS.mem_spec in Hcv; *)
-(*                  apply Hidi in Hcv; *)
-(*                  inversion 1; *)
-(*                  contradiction] *)
-(*           | H:PS.for_all _ _ = false |- _ => *)
-(*             apply not_for_all_spec in Hcv; [|apply check_var_compat] *)
-(*           | _ => idtac *)
-(*           end; *)
-(*           intro Hwsch'; *)
-(*           apply Hcv; *)
-(*           inversion_clear Hwsch' as [|? ? ? Hwsch0 HH *)
-(*                                         |? ? ? ? Hwsch0 HH *)
-(*                                         |? ? ? ? Hwsch0 Hi HH]; *)
-(*           intros x Hx; *)
-(*           apply free_in_caexp_spec in Hx || apply free_in_laexp_spec in Hx; *)
-(*           destruct Hx as [Hx|Hx]; [ | apply not_In_empty in Hx; contradiction ]; *)
-(*           intros; *)
-(*           repeat progress *)
-(*                  match goal with *)
-(*                  | |- _ /\ _ => split; intros *)
-(*                  | H: _ /\ _ |- _ => destruct H *)
-(*                  | H: Is_free_in_caexp _ _ |- _ => apply HH in H *)
-(*                  | H: Is_free_in_laexp _ _ |- _ => apply HH in H *)
-(*                  | |- check_var defined' variables' x = true *)
-(*                    => apply check_var_spec *)
-(*                  | H1:~PS.In ?x ?mems -> Is_variable_in ?x ?eqs, *)
-(*                    H2:~PS.In ?x ?mems |- PS.In ?x variables' *)
-(*                    => apply H1 in H2; apply Hivi in H2; assumption *)
-(*                  | H1:PS.In ?x ?mems -> ~Is_defined_in ?x ?eqs, *)
-(*                       H2:PS.In ?x ?mems |- _ => apply H1 in H2 *)
-(*                  | H:~Is_defined_in ?x ?eqs |- ~PS.In ?x defined' *)
-(*                    => intro HN; apply Hidi in HN; contradiction *)
-(*                  end); *)
-(*           rewrite Hivi; auto. *)
-(* Qed. *)
-(*      *) *)
-(*     Lemma well_sch_spec: *)
-(*       forall argIns eqns, *)
-(*         if well_sch argIns eqns *)
-(*         then Is_well_sch mems argIns eqns *)
-(*         else ~Is_well_sch mems argIns eqns. *)
-(*     Proof. *)
-(*       intros argIn eqns. *)
-(*       pose proof (well_sch_pre_spec argIn eqns). *)
-(*       unfold well_sch. *)
-(*       destruct (List.fold_right check_eq (true, PS.empty, fold_left (fun a b => PS.add b a) argIn PS.empty) eqns) *)
-(*         as [[good defined] variables]. *)
-(*       simpl. *)
-(*       specialize H with good defined variables. *)
-(*       pose proof (H (eq_refl _)) as H'; clear H. *)
-(*       destruct H' as [Ht Hf]. *)
-(*       destruct good; *)
-(*         intuition. *)
-(*     Qed. *)
+    Lemma in_fold_left_add:
+      forall x xs S,
+        PS.In x (fold_left (fun S' x => PS.add x S') xs S)
+        <->
+        In x xs \/ PS.In x S.
+    Proof.
+      induction xs as [|y xs IH].
+      split; intro H; simpl in *;
+        intuition.
+      intro S; split; intro H.
+      - apply IH in H.
+        destruct H.
+        now left; constructor (assumption).
+        apply PS.add_spec in H; simpl; intuition.
+      - simpl; apply IH; simpl in H; intuition.
+    Qed.
 
+    Lemma well_sch_pre_spec:
+      forall args eqs good defined variables,
+        (good, defined, variables)
+        = List.fold_right check_eq (true, PS.empty,
+                            fold_left (fun a b => PS.add b a) args PS.empty) eqs
+        ->
+        (good = true
+         -> (Is_well_sch mems args eqs
+             /\ (forall x, PS.In x defined <-> Is_defined_in_eqs x eqs)
+             /\ (forall x, PS.In x variables <->
+                              Is_variable_in_eqs x eqs \/ In x args)))
+        /\ (good = false -> ~Is_well_sch mems args eqs).
+    Proof.
+      induction eqs as [|eq].
+      - (* case nil: *)
+        simpl. injection 1. intros.
+        subst variables0; subst defined0; subst good.
+        intuition;
+          repeat match goal with
+                 | H:PS.In _ PS.empty |- _ => apply PS.empty_spec in H; contradiction
+                 | H:Is_defined_in_eqs _ nil |- _ => inversion H
+                 | H:Is_variable_in_eqs _ nil |- _ => inversion H
+                 | H: context[fold_left _ _ _] |- _ =>
+                   apply in_fold_left_add in H
+                 | _ => intuition
+                 end.
+        apply in_fold_left_add; auto.
+      - (* case cons: *)
+        intros good defined variables HH.
+        destruct (fold_right check_eq (true, PS.empty,
+                    fold_left (fun (a : PS.t) (b : positive) => PS.add b a)
+                              args PS.empty) eqs)
+          as [[good' defined'] variables'] eqn:Heq.
+        specialize IHeqs with good' defined' variables'.
+        pose proof (IHeqs (eq_refl (good', defined', variables'))) as IH;
+          clear IHeqs.
+        destruct IH as [IHt IHf].
+        split; intro Hg; rewrite Hg in *; clear Hg.
+        + (* good=true *)
+          simpl in HH; rewrite Heq in HH.
+          simpl in HH.
+          destruct good'; [|discriminate].
+          specialize (IHt eq_refl).
+          clear IHf; destruct IHt as [IHwsch [IHdef IHvar]].
+          injection HH; clear HH; intros Hv Hd H.
+          subst variables; subst defined.
+          symmetry in H.
+          apply Bool.andb_true_iff in H.
+          destruct H as [H1 H2].
+          apply PS.for_all_spec in H1; [|now apply check_var_compat].
+          apply Bool.negb_true_iff in H2.
+          apply mem_spec_false in H2.
+          split; [|split].
+          * (* Is_well_sch *)
+            constructor.
+            assumption.
+            intros x Hfree.
+            apply free_in_equation_spec' in Hfree.
+            apply H1 in Hfree.
+            apply check_var_spec in Hfree.
+            destruct Hfree as [Hfree1 Hfree2].
+            split; intro HH; (apply Hfree1 in HH || apply Hfree2 in HH).
+            intro Hdef; apply IHdef in Hdef; apply HH; assumption.
+            apply IHvar; assumption.
+            intros x Hdef Hdefs; apply IHdef in Hdefs.
+            apply Is_defined_in_eqs_var_defined in Hdef.
+            rewrite Hdef in *. auto.
+          * (* defined set *)
+            intro x; split; intro HH.
+            apply PS.add_spec in HH.
+            destruct HH as [HH|HH].
+            subst x; constructor; now apply Is_defined_in_eqs_var_defined.
+            apply IHdef in HH.
+            constructor (assumption).
+            apply PS.add_spec.
+            inversion_clear HH.
+            apply Is_defined_in_eqs_var_defined in H; subst x; auto.
+            right; apply IHdef; assumption.
+          * (* variables set *)
+            intro x; split; intro HH.
+            apply variable_eq_empty in HH.
+            destruct HH as [HH|HH].
+            destruct eq;
+              ((apply PS.add_spec in HH;
+                destruct HH as [HH|HH];
+                [subst i; left; now repeat constructor
+                |apply PS.empty_spec in HH; contradiction])
+               || apply PS.empty_spec in HH; contradiction).
+            apply IHvar in HH; intuition; left; constructor (assumption).
+            apply variable_eq_empty.
+            destruct HH as [HH|HH].
+            apply Is_variable_in_cons in HH.
+            destruct HH as [HH|HH]; [left|right].
+            destruct eq; inversion_clear HH; simpl; now intuition.
+            apply IHvar; intuition.
+            right; apply IHvar; auto.
+        + (* good=false *)
+          intro Hwsch.
+          simpl in HH; rewrite Heq in HH; clear Heq; simpl in HH.
+          destruct good'; [specialize (IHt eq_refl); clear IHf
+                          | specialize (IHf eq_refl);
+                            apply Is_well_sch_cons in Hwsch;
+                            apply IHf with (1:=Hwsch)].
+          destruct IHt as [_ [IHdef IHvar]].
+          injection HH; clear HH; intros Hv Hd HH.
+          subst variables; subst defined; symmetry in HH.
+          apply Bool.andb_false_iff in HH.
+          inversion_clear Hwsch as [|Ha Hb Hwschs Hfree Hdefd].
+          destruct HH as [HH|HH].
+          * (* check_var of free fails *)
+            apply not_for_all_spec in HH; [|apply check_var_compat].
+            apply HH; clear HH.
+            intros x HH.
+            apply free_in_equation_spec in HH.
+            destruct HH as [HH|HH]; [|apply PS.empty_spec in HH].
+            apply Hfree in HH.
+            destruct HH as [Hmem Hvar];
+              apply check_var_spec; split; intro HHm;
+                (specialize (Hmem HHm) || specialize (Hvar HHm)).
+            intro Hdef; apply IHdef in Hdef; apply Hmem; assumption.
+            apply IHvar; intuition.
+            contradiction.
+          * (* already defined *)
+            apply Bool.negb_false_iff in HH.
+            rewrite PS.mem_spec in HH.
+            apply Hdefd with (i:=var_defined eq).
+            apply Is_defined_in_eqs_var_defined; reflexivity.
+            apply IHdef; assumption.
+    Qed.
+    
+    Lemma well_sch_spec:
+      forall args eqns,
+        if well_sch args eqns
+        then Is_well_sch mems args eqns
+        else ~Is_well_sch mems args eqns.
+    Proof.
+      intros args eqns.
+      pose proof (well_sch_pre_spec args eqns).
+      unfold well_sch.
+      destruct (fold_right check_eq
+                  (true, PS.empty,
+                   fold_left (fun a b => PS.add b a) args PS.empty) eqns)
+        as [[good defined] variables].
+      simpl.
+      specialize H with good defined variables.
+      pose proof (H (eq_refl _)) as H'; clear H.
+      destruct H' as [Ht Hf].
+      destruct good;
+        intuition.
+    Qed.
+
+    Lemma Is_well_sch_by_refl:
+      forall args eqns,
+        well_sch args eqns = true <-> Is_well_sch mems args eqns.
+    Proof.
+      intros args eqns.
+      pose proof (well_sch_spec args eqns) as Hwss.
+      split; intro H.
+      rewrite H in Hwss; assumption.
+      destruct (well_sch args eqns); [reflexivity|].
+      exfalso; apply Hwss; apply H.
+    Qed.
+    
+    Lemma well_sch_dec:
+      forall args eqns,
+        {Is_well_sch mems args eqns}+{~Is_well_sch mems args eqns}.
+    Proof.
+      intros args eqns.
+      pose proof (well_sch_spec args eqns) as Hwss.
+      destruct (well_sch args eqns); [left|right]; assumption.
+    Qed.
+    
   End Decide.
 
-End DecideFun.
+End DECIDE.
+
+Module Decide
+       (Ids           : IDS)
+       (Op            : OPERATORS)
+       (Import Syn    : SYNTAX Ids Op)
+       (IsF           : ISFREE Ids Op Syn)
+       (Import IsFDec : IsFree.Decide.DECIDE Ids Op Syn IsF)
+       (Import Ord    : ORDERED Ids Op Syn)
+       (Import Mem    : MEMORIES Ids Op Syn)
+       (Import IsD    : ISDEFINED Ids Op Syn Mem)
+       (Import IsV    : ISVARIABLE Ids Op Syn Mem IsD)
+       (Import IsDDec : IsDefined.Decide.DECIDE Ids Op Syn Mem IsD)
+       (Import IsVDec : IsVariable.Decide.DECIDE Ids Op Syn Mem IsD IsV)
+       (Import NoD    : NODUP Ids Op Syn Mem IsD IsV)
+       (Import Wef    : WELLFORMED Ids Op Syn IsF Ord Mem IsD IsV NoD)
+       <: DECIDE Ids Op Syn IsF IsFDec Ord Mem IsD IsV IsDDec IsVDec NoD Wef.
+  
+  Include DECIDE Ids Op Syn IsF IsFDec Ord Mem IsD IsV IsDDec IsVDec NoD Wef.
+End Decide.
+  
